Add manual and automatic translations of Rocq

lava/out/Benchmark/PLE/MonadMaybe.v
@@ -1,393 +1,238 @@
 From coqDeps Require Export LiquidPreludeUtil.
 Open Scope Z_scope.
 Open Scope Int_scope.
-From Coq Require Import Unicode.Utf8.
-Ltac solver := quicksolve.
-
-Inductive MaybeInt_u: Set :=
-  | Just_u: Z → MaybeInt_u | Nothing_u: MaybeInt_u.
-
-Fixpoint MaybeInt_eq (x y : MaybeInt_u): bool :=
-  match (x, y) with
-  | (Just_u VV, Just_u VV') => true && (VV ==? VV')
-  | (Nothing_u, Nothing_u) => true
-  | (_, _) => false
-  end.
-
-Definition MaybeInt_eq_refl : ∀ (x : MaybeInt_u), is_true (MaybeInt_eq x x).
-Proof.
-  eq_refl.
-Qed.
-
-#[global] Hint Resolve MaybeInt_eq_refl: eq_hint_db.
-
-Definition MaybeInt_eqb_eq : ∀ (s t : MaybeInt_u), is_true (MaybeInt_eq s t) → s = t.
-Proof.
-  eqb_eq_lem.
-Qed.
-
-#[global] Hint Resolve MaybeInt_eqb_eq: eq_hint_db.
-
-#[global] Instance leibnitz_eq_MaybeInt: LeibnitzEqB := {
-    equalB' := MaybeInt_eq;
-    refl' := MaybeInt_eq_refl;
-    eqb_eq' := MaybeInt_eqb_eq }.
-
-Fixpoint MaybeInt_wf (x : MaybeInt_u): Prop :=
-  match x with | Just_u VV => True | Nothing_u => True end.
-
-Theorem MaybeInt_wf_ref [p : MaybeInt_u → Prop] (tm : {v: MaybeInt_u | MaybeInt_wf v ∧ p v}):
-  MaybeInt_wf ⌊ tm ⌋.
-Proof.
-  destruct tm as [tm tm_p]. solver.
-Qed.
-
-Global Notation MaybeInt := {x: MaybeInt_u | MaybeInt_wf x ∧ True}.
-
-Definition Just_lem (VV : {VV: Z | True}): MaybeInt_wf (Just_u ⌊ VV ⌋) ∧ True.
-Proof.
-  repeat first [split; solver].
+Set Universe Polymorphism.
+Inductive MaybeInt_u : Type := 
+	 | Just_u: Z -> MaybeInt_u
+	 | Nothing_u: MaybeInt_u. 
+Fixpoint MaybeInt_eq (x: MaybeInt_u) (y: MaybeInt_u): bool := 
+	match (x, y) with (Just_u x, Just_u x') => (true && (x ==? x')) | (Nothing_u, Nothing_u) => true | (_, _) => false end. 
+Theorem MaybeInt_eq_refl: (forall (x: MaybeInt_u) , is_true (MaybeInt_eq x x)). 
+Proof. 
+	eq_refl_rec. 
+Qed. 
+#[global] Hint Resolve MaybeInt_eq_refl : eq_hint_db.
+Theorem MaybeInt_eqb_eq: (forall (s: MaybeInt_u) (t: MaybeInt_u) , (is_true (MaybeInt_eq s t)) -> (s = t)). 
+Proof. 
+	eqb_eq_lem. 
+Qed. 
+#[global] Hint Resolve MaybeInt_eqb_eq : eq_hint_db.
+#[global] Instance leibnitz_eq_MaybeInt : LeibnitzEqB := { 
+	equalB' := MaybeInt_eq;
+	refl' := MaybeInt_eq_refl;
+	eqb_eq' := MaybeInt_eqb_eq
+}.
+Fixpoint MaybeInt_wf (x: MaybeInt_u): Prop := 
+	match x with (Just_u VV) => True | Nothing_u => True end. 
+Theorem MaybeInt_wf_ref [p: MaybeInt_u -> Prop] (tm: {v: MaybeInt_u | (MaybeInt_wf v) /\ (p v)}): MaybeInt_wf (⌊ tm -⌋). 
+Proof. 
+	destruct tm as [tm tm_p]. 
+	solver. 
+Qed. 
+Global Notation MaybeInt := {x: MaybeInt_u | (MaybeInt_wf x) /\ True}. 
+Definition Just_lem (VV: {VV: Z | True}): (MaybeInt_wf (Just_u (⌊ VV -⌋))) /\ True. 
+Proof. 
+	repeat first [split; solver]. 
+Defined. 
+Definition Just (VV: {VV: Z | True}): MaybeInt := 
+	exist _ (Just_u (⌊ VV -⌋)) (Just_lem VV). 
+Definition Nothing_lem: (MaybeInt_wf Nothing_u) /\ True. 
+Proof. 
+	repeat first [split; solver]. 
+Defined. 
+Definition Nothing: MaybeInt := 
+	exist _ Nothing_u Nothing_lem. 
+#[global] Hint Resolve MaybeInt_wf_ref : wf_constr_db.
+#[global] Hint Unfold MaybeInt_wf : wf_constr_db.
+#[global] Hint Resolve MaybeInt_eq : ref_constr_db.
+#[global] Hint Unfold Just : ref_constr_db.
+#[global] Hint Unfold Nothing : ref_constr_db.
+Definition bind_spec (lq_tmp0: MaybeInt) (lq_tmp1: (@Pack ({lq_tmp2: Z | True} ::RT (fun (lq_tmp2: {lq_tmp2: Z | True}) => nilRT)) (Z ::UT nilUT) (ltac: (mkProjectsArgListTG ({lq_tmp2: Z | True} ::RT (fun (lq_tmp2: {lq_tmp2: Z | True}) => nilRT)) (Z ::UT nilUT))) MaybeInt_u (fun (x_61572807: (ArgList {lq_tmp2: Z | True} ::RT (fun (lq_tmp2: {lq_tmp2: Z | True}) => nilRT))) => (fun (v_x_61572807: MaybeInt_u) => (ltac: (flattenP (fun (lq_tmp2: {lq_tmp2: Z | True}) => (fun (VV: MaybeInt_u) => ((MaybeInt_wf VV) /\ True))) x_61572807 v_x_61572807)))))): Type := 
+	MaybeInt. 
+#[global] Hint Unfold bind_spec : lia_unfold.
+Definition bind (lq_tmp0: MaybeInt) (lq_tmp1: (@Pack ({lq_tmp2: Z | True} ::RT (fun (lq_tmp2: {lq_tmp2: Z | True}) => nilRT)) (Z ::UT nilUT) (ltac: (mkProjectsArgListTG ({lq_tmp2: Z | True} ::RT (fun (lq_tmp2: {lq_tmp2: Z | True}) => nilRT)) (Z ::UT nilUT))) MaybeInt_u (fun (x_61572807: (ArgList {lq_tmp2: Z | True} ::RT (fun (lq_tmp2: {lq_tmp2: Z | True}) => nilRT))) => (fun (v_x_61572807: MaybeInt_u) => (ltac: (flattenP (fun (lq_tmp2: {lq_tmp2: Z | True}) => (fun (VV: MaybeInt_u) => ((MaybeInt_wf VV) /\ True))) x_61572807 v_x_61572807)))))): bind_spec lq_tmp0 lq_tmp1. 
+Proof. 
+	destruct lq_tmp0 as [lq_tmp0 lq_tmp0_p]. 
+	try revert lq_tmp1_p; generalize dependent lq_tmp1; 
+	induction lq_tmp0 as [(*Just*) m | (*Nothing*) ]. 
+	  - intros . 
+		refine (subsumptionCast _ _ 
+		((getPackF lq_tmp1) (exist (fun (lq_tmp2: Z) => True) m (ltac: (solver)))) _); 
+		solver.  
+	  - intros . 
+		refine (subsumptionCast _ _ Nothing _); 
+		solver.  
+Defined. 
+Inductive bind_rel : (MaybeInt_u -> ((@uPack (Z ::UT nilUT) MaybeInt_u) -> (MaybeInt_u -> Prop))) := 
+	 | bind_Nothing: (forall (lq_tmp1: @uPack (Z ::UT nilUT) MaybeInt_u) , bind_rel Nothing_u lq_tmp1 Nothing_u)
+	 | bind_Just: (forall (lq_tmp1: @uPack (Z ::UT nilUT) MaybeInt_u) m , forall (lq_tmp1res: _), ((getUPackRel lq_tmp1) m lq_tmp1res) -> (bind_rel (Just_u m) lq_tmp1 lq_tmp1res)). 
+#[global] Hint Constructors bind_rel : core_hint_db.
+#[global] Instance bind_lookup_rel : dictionary rel bind := { 
+	lookup' := bind_rel
+}.
+#[global] Instance bind_getF : getFunc bind_rel := { 
+	getF' := bind
+}.
+Theorem bind_rel_funct [lq_tmp0: MaybeInt_u] [lq_tmp1: @uPack (Z ::UT nilUT) MaybeInt_u]: (forall (VV: MaybeInt_u) (VV': MaybeInt_u) (H: bind_rel lq_tmp0 lq_tmp1 VV) (K: bind_rel lq_tmp0 lq_tmp1 VV') , VV = VV'). 
+Proof. 
+	try revert lq_tmp1_p; generalize dependent lq_tmp1; 
+	induction lq_tmp0 as [(*Just*) m | (*Nothing*) ]; 
+	intros ; 
+	rel_functionhood_body. 
+Qed. 
+#[global] Hint Resolve bind_rel_funct : f_rel_funct_db.
+Theorem bind_Nothing_lem (lq_tmp1: @uPack (Z ::UT nilUT) MaybeInt_u): (bind_rel Nothing_u lq_tmp1 Nothing_u) <-> True. 
+Proof. 
+	rel_back' ( _nil). 
+Qed. 
+#[global] Hint Rewrite bind_Nothing_lem : f_rel_back.
+Theorem bind_Just_lem (m: _) (lq_tmp1: @uPack (Z ::UT nilUT) MaybeInt_u) (lq_tmp1res: _) (h_48917519: (getUPackRel lq_tmp1) m lq_tmp1res): (bind_rel (Just_u m) lq_tmp1 lq_tmp1res) <-> True. 
+Proof. 
+	rel_back' ( _nil). 
+Qed. 
+#[global] Hint Rewrite bind_Just_lem : f_rel_back.
+Theorem bind_rel_ex (lq_tmp0: MaybeInt_u) (lq_tmp1: (@Pack ({lq_tmp2: Z | True} ::RT (fun (lq_tmp2: {lq_tmp2: Z | True}) => nilRT)) (Z ::UT nilUT) (ltac: (mkProjectsArgListTG ({lq_tmp2: Z | True} ::RT (fun (lq_tmp2: {lq_tmp2: Z | True}) => nilRT)) (Z ::UT nilUT))) MaybeInt_u (fun (x_61572807: (ArgList {lq_tmp2: Z | True} ::RT (fun (lq_tmp2: {lq_tmp2: Z | True}) => nilRT))) => (fun (v_x_61572807: MaybeInt_u) => (ltac: (flattenP (fun (lq_tmp2: {lq_tmp2: Z | True}) => (fun (VV: MaybeInt_u) => ((MaybeInt_wf VV) /\ True))) x_61572807 v_x_61572807)))))) (lq_tmp0_p: (MaybeInt_wf lq_tmp0) /\ True): bind_rel lq_tmp0 (packProj lq_tmp1) (⌊ bind (exist _ lq_tmp0 lq_tmp0_p) lq_tmp1 -⌋). 
+Proof. 
+	Opaque bind.
+	existence_lemma_pre bind; 
+	try revert lq_tmp1_p; generalize dependent lq_tmp1; 
+	induction lq_tmp0 as [(*Just*) m | (*Nothing*) ]; 
+	intros ; 
+	[fix_notations| 
+	fix_notations]; 
+	simpl in *. 
+	Transparent bind.
+	all: existence_lemma_quicksolve bind; 
+	f__f_rel_ex_body; 
+	f_rel_finish. 
+Qed. 
+#[global] Hint Resolve bind_rel_ex : rel_ax_db.
+#[global] Opaque bind. 
+Theorem bind__bind_rel_rw (lq_tmp0: MaybeInt_u) (lq_tmp1: (@Pack ({lq_tmp2: Z | True} ::RT (fun (lq_tmp2: {lq_tmp2: Z | True}) => nilRT)) (Z ::UT nilUT) (ltac: (mkProjectsArgListTG ({lq_tmp2: Z | True} ::RT (fun (lq_tmp2: {lq_tmp2: Z | True}) => nilRT)) (Z ::UT nilUT))) MaybeInt_u (fun (x_61572807: (ArgList {lq_tmp2: Z | True} ::RT (fun (lq_tmp2: {lq_tmp2: Z | True}) => nilRT))) => (fun (v_x_61572807: MaybeInt_u) => (ltac: (flattenP (fun (lq_tmp2: {lq_tmp2: Z | True}) => (fun (VV: MaybeInt_u) => ((MaybeInt_wf VV) /\ True))) x_61572807 v_x_61572807)))))) (lq_tmp0_p: (MaybeInt_wf lq_tmp0) /\ True) (VV: MaybeInt_u): ((⌊ bind (exist _ lq_tmp0 lq_tmp0_p) lq_tmp1 -⌋) = VV) <-> (bind_rel lq_tmp0 (packProj lq_tmp1) VV). 
+Proof. 
+	f__f_rel_rw. 
+Qed. 
+#[global] Hint Rewrite bind__bind_rel_rw : f_rel_funct_db.
+#[global] Hint Resolve bind__bind_rel_rw : rel_ax_db.
+#[global] Instance bind_lookup_rw : dictionary rwLem bind := { 
+	lookup' := bind__bind_rel_rw
+}.
+Theorem bind__bind_rel (lq_tmp0_r: MaybeInt) (lq_tmp1_r: (@Pack ({lq_tmp2: Z | True} ::RT (fun (lq_tmp2: {lq_tmp2: Z | True}) => nilRT)) (Z ::UT nilUT) (ltac: (mkProjectsArgListTG ({lq_tmp2: Z | True} ::RT (fun (lq_tmp2: {lq_tmp2: Z | True}) => nilRT)) (Z ::UT nilUT))) MaybeInt_u (fun (x_61572807: (ArgList {lq_tmp2: Z | True} ::RT (fun (lq_tmp2: {lq_tmp2: Z | True}) => nilRT))) => (fun (v_x_61572807: MaybeInt_u) => (ltac: (flattenP (fun (lq_tmp2: {lq_tmp2: Z | True}) => (fun (VV: MaybeInt_u) => ((MaybeInt_wf VV) /\ True))) x_61572807 v_x_61572807)))))) (VV: MaybeInt_u): ((⌊ bind lq_tmp0_r lq_tmp1_r -⌋) = VV) <-> (bind_rel (⌊ lq_tmp0_r -⌋) (packProj lq_tmp1_r) VV). 
+Proof. 
+	f__f_rel. 
+Qed. 
+#[global] Hint Rewrite bind__bind_rel : f_rel_funct_db.
+Theorem bind__bind_rel' (lq_tmp0: MaybeInt_u) (lq_tmp1: @uPack (Z ::UT nilUT) MaybeInt_u) (lq_tmp0_r: MaybeInt) (lq_tmp1_r: (@Pack ({lq_tmp2: Z | True} ::RT (fun (lq_tmp2: {lq_tmp2: Z | True}) => nilRT)) (Z ::UT nilUT) (ltac: (mkProjectsArgListTG ({lq_tmp2: Z | True} ::RT (fun (lq_tmp2: {lq_tmp2: Z | True}) => nilRT)) (Z ::UT nilUT))) MaybeInt_u (fun (x_61572807: (ArgList {lq_tmp2: Z | True} ::RT (fun (lq_tmp2: {lq_tmp2: Z | True}) => nilRT))) => (fun (v_x_61572807: MaybeInt_u) => (ltac: (flattenP (fun (lq_tmp2: {lq_tmp2: Z | True}) => (fun (VV: MaybeInt_u) => ((MaybeInt_wf VV) /\ True))) x_61572807 v_x_61572807)))))) (VV: MaybeInt_u): (lq_tmp0 = (⌊ lq_tmp0_r -⌋)) -> ((lq_tmp1 = (packProj lq_tmp1_r)) -> (((⌊ bind lq_tmp0_r lq_tmp1_r -⌋) = VV) <-> (bind_rel lq_tmp0 lq_tmp1 VV))). 
+Proof. 
+	intros -> ->. 
+	refine (bind__bind_rel lq_tmp0_r lq_tmp1_r VV). 
+Qed. 
+#[global] Hint Resolve bind__bind_rel' : f_rel_funct_db.
+Theorem bind_rel_mk [lq_tmp0: MaybeInt_u] [lq_tmp1: (@Pack ({lq_tmp2: Z | True} ::RT (fun (lq_tmp2: {lq_tmp2: Z | True}) => nilRT)) (Z ::UT nilUT) (ltac: (mkProjectsArgListTG ({lq_tmp2: Z | True} ::RT (fun (lq_tmp2: {lq_tmp2: Z | True}) => nilRT)) (Z ::UT nilUT))) MaybeInt_u (fun (x_61572807: (ArgList {lq_tmp2: Z | True} ::RT (fun (lq_tmp2: {lq_tmp2: Z | True}) => nilRT))) => (fun (v_x_61572807: MaybeInt_u) => (ltac: (flattenP (fun (lq_tmp2: {lq_tmp2: Z | True}) => (fun (VV: MaybeInt_u) => ((MaybeInt_wf VV) /\ True))) x_61572807 v_x_61572807)))))] (lq_tmp0_p: (MaybeInt_wf lq_tmp0) /\ True): {VV: _ | bind_rel lq_tmp0 (packProj lq_tmp1) VV}. 
+Proof. 
+	intros ; 
+	refine (subsumptionCast _ (fun (VV: _) => (bind_rel lq_tmp0 (packProj lq_tmp1) VV)) (bind (exist _ lq_tmp0 lq_tmp0_p) lq_tmp1) _); 
+	rewrite <- bind__bind_rel'; 
+	quicksolve. 
+Qed. 
+#[global] Hint Resolve bind_rel_mk : f_rel_funct_db.
+Definition retrn_spec (lq_tmp0: {lq_tmp0: Z | True}): Type := 
+	MaybeInt. 
+#[global] Hint Unfold retrn_spec : lia_unfold.
+Definition retrn (lq_tmp0: {lq_tmp0: Z | True}): retrn_spec lq_tmp0. 
+Proof. 
+	destruct lq_tmp0 as [lq_tmp0 lq_tmp0_p]. 
+	refine (subsumptionCast _ _ 
+		(Just (exist (fun (VV: Z) => True) lq_tmp0 (ltac: (solver)))) _); 
+	solver. 
+Defined. 
+Inductive retrn_rel : (Z -> (MaybeInt_u -> Prop)) := 
+	 | retrn_def: (forall lq_tmp0 , retrn_rel lq_tmp0 (Just_u lq_tmp0)). 
+#[global] Hint Constructors retrn_rel : core_hint_db.
+#[global] Instance retrn_lookup_rel : dictionary rel retrn := { 
+	lookup' := retrn_rel
+}.
+#[global] Instance retrn_getF : getFunc retrn_rel := { 
+	getF' := retrn
+}.
+Theorem retrn_rel_funct [lq_tmp0: Z]: (forall (VV: MaybeInt_u) (VV': MaybeInt_u) (H: retrn_rel lq_tmp0 VV) (K: retrn_rel lq_tmp0 VV') , VV = VV'). 
+Proof. 
+	rel_functionhood_body. 
+Qed. 
+#[global] Hint Resolve retrn_rel_funct : f_rel_funct_db.
+Theorem retrn_def_lem (lq_tmp0: _): (retrn_rel lq_tmp0 (Just_u lq_tmp0)) <-> True. 
+Proof. 
+	rel_back' ( _nil). 
+Qed. 
+#[global] Hint Rewrite retrn_def_lem : f_rel_back.
+Theorem retrn_rel_ex (lq_tmp0: Z) (lq_tmp0_p: True): retrn_rel lq_tmp0 (⌊ retrn (exist _ lq_tmp0 lq_tmp0_p) -⌋). 
+Proof. 
+	Opaque retrn.
+	existence_lemma_pre retrn; 
+	fix_notations; 
+	simpl in *. 
+	Transparent retrn.
+	all: existence_lemma_quicksolve retrn; 
+	f__f_rel_ex_body; 
+	f_rel_finish. 
+Qed. 
+#[global] Hint Resolve retrn_rel_ex : rel_ax_db.
+#[global] Opaque retrn. 
+Theorem retrn__retrn_rel_rw (lq_tmp0: Z) (lq_tmp0_p: True) (VV: MaybeInt_u): ((⌊ retrn (exist _ lq_tmp0 lq_tmp0_p) -⌋) = VV) <-> (retrn_rel lq_tmp0 VV). 
+Proof. 
+	f__f_rel_rw. 
+Qed. 
+#[global] Hint Rewrite retrn__retrn_rel_rw : f_rel_funct_db.
+#[global] Hint Resolve retrn__retrn_rel_rw : rel_ax_db.
+#[global] Instance retrn_lookup_rw : dictionary rwLem retrn := { 
+	lookup' := retrn__retrn_rel_rw
+}.
+Theorem retrn__retrn_rel (lq_tmp0_r: {lq_tmp0: Z | True}) (VV: MaybeInt_u): ((⌊ retrn lq_tmp0_r -⌋) = VV) <-> (retrn_rel (⌊ lq_tmp0_r -⌋) VV). 
+Proof. 
+	f__f_rel. 
+Qed. 
+#[global] Hint Rewrite retrn__retrn_rel : f_rel_funct_db.
+Theorem retrn__retrn_rel' (lq_tmp0: Z) (lq_tmp0_r: {lq_tmp0: Z | True}) (VV: MaybeInt_u): (lq_tmp0 = (⌊ lq_tmp0_r -⌋)) -> (((⌊ retrn lq_tmp0_r -⌋) = VV) <-> (retrn_rel lq_tmp0 VV)). 
+Proof. 
+	intros ->. 
+	refine (retrn__retrn_rel lq_tmp0_r VV). 
+Qed. 
+#[global] Hint Resolve retrn__retrn_rel' : f_rel_funct_db.
+Theorem retrn_rel_mk [lq_tmp0: Z] (lq_tmp0_p: True): {VV: _ | retrn_rel lq_tmp0 VV}. 
+Proof. 
+	intros ; 
+	refine (subsumptionCast _ (fun (VV: _) => (retrn_rel lq_tmp0 VV)) (retrn (exist _ lq_tmp0 lq_tmp0_p)) _); 
+	rewrite <- retrn__retrn_rel'; 
+	quicksolve. 
+Qed. 
+#[global] Hint Resolve retrn_rel_mk : f_rel_funct_db.
+#[global] Instance retrnPack : (@Pack ({lq_tmp0: Z | True} ::RT (fun (lq_tmp0_r: {lq_tmp0: Z | True}) => nilRT)) (Z ::UT nilUT) (ltac: (mkProjectsArgListTG ({lq_tmp0: Z | True} ::RT (fun (lq_tmp0_r: {lq_tmp0: Z | True}) => nilRT)) (Z ::UT nilUT))) MaybeInt_u (fun (x_89043232: (ArgList {lq_tmp0: Z | True} ::RT (fun (lq_tmp0_r: {lq_tmp0: Z | True}) => nilRT))) => (fun (v_x_89043232: MaybeInt_u) => (ltac: (flattenP (fun (lq_tmp0_r: {lq_tmp0: Z | True}) => (fun (VV: MaybeInt_u) => ((MaybeInt_wf VV) /\ True))) x_89043232 v_x_89043232))))).
+Proof. 
+	buildPackG retrn retrn_rel retrn__retrn_rel retrn_rel_funct. 
 Defined.
-
-Definition Just (VV : {VV: Z | True}): MaybeInt :=
-  exist _ (Just_u ⌊ VV ⌋) (Just_lem VV).
-
-Definition Nothing_lem : MaybeInt_wf Nothing_u ∧ True.
-Proof.
-  repeat first [split; solver].
-Defined.
-
-Definition Nothing : MaybeInt :=
-  exist _ Nothing_u Nothing_lem.
-
-#[global] Hint Resolve MaybeInt_wf_ref: wf_constr_db.
-
-#[global] Hint Unfold MaybeInt_wf: wf_constr_db.
-
-#[global] Hint Resolve MaybeInt_eq: ref_constr_db.
-
-#[global] Hint Unfold Just: ref_constr_db.
-
-#[global] Hint Unfold Nothing: ref_constr_db.
-
-Definition bind
-  (lq_tmp0 : MaybeInt)
-  (lq_tmp2 : @Pack
-             ({VV: Z | True} ::RT λ (lq_tmp2 : {VV: Z | True}), nilRT)
-             (Z ::UT nilUT)
-             ltac:(mkProjectsArgListTG (({VV: Z | True} ::RT λ (lq_tmp2 : {VV: Z | True}), nilRT)) ((Z ::UT nilUT)))
-             MaybeInt_u
-             (λ (x_10329927 : ArgList ({VV: Z | True} ::RT λ (lq_tmp2 : {VV: Z | True}), nilRT))
-                (v_x_10329927 : MaybeInt_u),
-              ltac:(flattenP (λ (lq_tmp2 : {VV: Z | True}) (VV : MaybeInt_u),
- MaybeInt_wf VV ∧ True) x_10329927 v_x_10329927))):
-  MaybeInt.
-Proof.
-  destruct lq_tmp0 as [lq_tmp0 lq_tmp0_p].
-  destruct lq_tmp0 as [m|].
-  - refine (getPackF lq_tmp2 (# m)).
-  - refine Nothing.
-Defined.
-
-Inductive bind_rel: MaybeInt_u → @uPack (Z ::UT nilUT) MaybeInt_u → MaybeInt_u → Prop :=
-  | bind_Nothing_x: ∀ (lq_tmp2 : @uPack (Z ::UT nilUT) MaybeInt_u),
-                    bind_rel Nothing_u lq_tmp2 Nothing_u
-  | bind_Just_x: ∀ m (lq_tmp2 : @uPack (Z ::UT nilUT) MaybeInt_u) lq_tmp2_res,
-                 getUPackRel lq_tmp2 m lq_tmp2_res → bind_rel (Just_u m) lq_tmp2 lq_tmp2_res.
-
-#[global] Hint Constructors bind_rel: core_hint_db.
-
-#[global] Instance bind_lookup_rel: dictionary rel bind := { lookup' := bind_rel }.
-
-#[global] Instance bind_getF: getFunc bind_rel := { getF' := bind }.
-
-Definition bind_rel_funct [lq_tmp0 : MaybeInt_u] [lq_tmp2 : @uPack (Z ::UT nilUT) MaybeInt_u]:
-  ∀ (VV VV' : MaybeInt_u), bind_rel lq_tmp0 lq_tmp2 VV → (bind_rel lq_tmp0 lq_tmp2 VV' → VV = VV').
-Proof.
-  destruct lq_tmp0 as [m|]; rel_functionhood_body.
-Qed.
-
-#[global] Hint Resolve bind_rel_funct: f_rel_funct_db.
-
-Theorem bind_Nothing_x_lem lq_tmp2 bind_Nothing_x_lem_res:
-  bind_rel Nothing_u lq_tmp2 bind_Nothing_x_lem_res ↔ bind_Nothing_x_lem_res == Nothing_u.
-Proof.
-  rel_back' _nil.
-Qed.
-
-#[global] Hint Rewrite bind_Nothing_x_lem: f_rel_back.
-
-Theorem bind_Just_x_lem lq_tmp2 m bind_Just_x_lem_res:
-  bind_rel (Just_u m) lq_tmp2 bind_Just_x_lem_res
-  ↔ ∃ lq_tmp2_res, getUPackRel lq_tmp2 m lq_tmp2_res ∧ bind_Just_x_lem_res == lq_tmp2_res.
-Proof.
-  rel_back' _nil.
-Qed.
-
-#[global] Hint Rewrite bind_Just_x_lem: f_rel_back.
-
-Theorem bind_rel_ex
-  (lq_tmp0 : MaybeInt_u)
-  (lq_tmp0_p : MaybeInt_wf lq_tmp0 ∧ True)
-  (lq_tmp2 : @Pack
-             ({lq_tmp2: Z | True} ::RT λ (lq_tmp2 : {lq_tmp2: Z | True}), nilRT)
-             (Z ::UT nilUT)
-             ltac:(mkProjectsArgListTG (({lq_tmp2: Z | True}
-  ::RT λ (lq_tmp2 : {lq_tmp2: Z | True}), nilRT)) ((Z ::UT nilUT)))
-             MaybeInt_u
-             (λ (x_82647028 : ArgList ({lq_tmp2: Z | True} ::RT λ (lq_tmp2 : {lq_tmp2: Z | True}), nilRT))
-                (v_x_82647028 : MaybeInt_u),
-              ltac:(flattenP (λ (lq_tmp2 : {lq_tmp2: Z | True}) (VV : MaybeInt_u),
- MaybeInt_wf VV ∧ True) x_82647028 v_x_82647028))):
-  bind_rel lq_tmp0 ⌊ lq_tmp2 ⌋ ⌊ bind (exist _ lq_tmp0 lq_tmp0_p) lq_tmp2 ⌋.
-Proof.
-  existence_lemma_pre bind;
-  destruct lq_tmp0 as [m|];
-  [fix_notations | fix_notations];
-  existence_lemma_quicksolve bind;
-  f__f_rel_ex_body;
-  f_rel_finish.
-Qed.
-
-#[global] Hint Resolve bind_rel_ex: rel_ax_db.
-
-Opaque bind.
-
-Theorem bind__bind_rel_rw
-  (lq_tmp0 : MaybeInt_u)
-  (lq_tmp0_p : MaybeInt_wf lq_tmp0 ∧ True)
-  (lq_tmp2 : @Pack
-             ({lq_tmp2: Z | True} ::RT λ (lq_tmp2 : {lq_tmp2: Z | True}), nilRT)
-             (Z ::UT nilUT)
-             ltac:(mkProjectsArgListTG (({lq_tmp2: Z | True}
-  ::RT λ (lq_tmp2 : {lq_tmp2: Z | True}), nilRT)) ((Z ::UT nilUT)))
-             MaybeInt_u
-             (λ (x_82647028 : ArgList ({lq_tmp2: Z | True} ::RT λ (lq_tmp2 : {lq_tmp2: Z | True}), nilRT))
-                (v_x_82647028 : MaybeInt_u),
-              ltac:(flattenP (λ (lq_tmp2 : {lq_tmp2: Z | True}) (VV : MaybeInt_u),
- MaybeInt_wf VV ∧ True) x_82647028 v_x_82647028)))
-  (VV : MaybeInt_u):
-  ⌊ bind (exist _ lq_tmp0 lq_tmp0_p) lq_tmp2 ⌋ = VV ↔ bind_rel lq_tmp0 ⌊ lq_tmp2 ⌋ VV.
-Proof.
-  f__f_rel_rw.
-Qed.
-
-#[global] Hint Rewrite bind__bind_rel_rw: f_rel_funct_db.
-
-#[global] Hint Resolve bind__bind_rel_rw: rel_ax_db.
-
-#[global] Instance bind_lookup_rw: dictionary rwLem bind := { lookup' := bind__bind_rel_rw }.
-
-Theorem bind__bind_rel
-  (lq_tmp0 : MaybeInt)
-  (lq_tmp2 : @Pack
-             ({VV: Z | True} ::RT λ (lq_tmp2 : {VV: Z | True}), nilRT)
-             (Z ::UT nilUT)
-             ltac:(mkProjectsArgListTG (({VV: Z | True} ::RT λ (lq_tmp2 : {VV: Z | True}), nilRT)) ((Z ::UT nilUT)))
-             MaybeInt_u
-             (λ (x_10329927 : ArgList ({VV: Z | True} ::RT λ (lq_tmp2 : {VV: Z | True}), nilRT))
-                (v_x_10329927 : MaybeInt_u),
-              ltac:(flattenP (λ (lq_tmp2 : {VV: Z | True}) (VV : MaybeInt_u),
- MaybeInt_wf VV ∧ True) x_10329927 v_x_10329927)))
-  (VV : MaybeInt_u):
-  ⌊ bind lq_tmp0 lq_tmp2 ⌋ = VV ↔ bind_rel ⌊ lq_tmp0 ⌋ ⌊ lq_tmp2 ⌋ VV.
-Proof.
-  f__f_rel.
-Qed.
-
-#[global] Hint Rewrite bind__bind_rel: f_rel_funct_db.
-
-Theorem bind__bind_rel'
-  (lq_tmp0_u : MaybeInt_u)
-  (lq_tmp2_u : @uPack (Z ::UT nilUT) MaybeInt_u)
-  (lq_tmp0 : MaybeInt)
-  (lq_tmp2 : @Pack
-             ({VV: Z | True} ::RT λ (lq_tmp2 : {VV: Z | True}), nilRT)
-             (Z ::UT nilUT)
-             ltac:(mkProjectsArgListTG (({VV: Z | True} ::RT λ (lq_tmp2 : {VV: Z | True}), nilRT)) ((Z ::UT nilUT)))
-             MaybeInt_u
-             (λ (x_10329927 : ArgList ({VV: Z | True} ::RT λ (lq_tmp2 : {VV: Z | True}), nilRT))
-                (v_x_10329927 : MaybeInt_u),
-              ltac:(flattenP (λ (lq_tmp2 : {VV: Z | True}) (VV : MaybeInt_u),
- MaybeInt_wf VV ∧ True) x_10329927 v_x_10329927)))
-  (VV : MaybeInt_u):
-  lq_tmp0_u = ⌊ lq_tmp0 ⌋
-  → (lq_tmp2_u = ⌊ lq_tmp2 ⌋ → ⌊ bind lq_tmp0 lq_tmp2 ⌋ = VV ↔ bind_rel lq_tmp0_u lq_tmp2_u VV).
-Proof.
-  intros -> ->. refine (bind__bind_rel lq_tmp0 lq_tmp2 VV).
-Qed.
-
-#[global] Hint Resolve bind__bind_rel': f_rel_funct_db.
-
-Definition bind_rel_mk
-  (lq_tmp0 : MaybeInt_u)
-  (lq_tmp0_p : MaybeInt_wf lq_tmp0 ∧ True)
-  (lq_tmp2 : @Pack
-             ({lq_tmp2: Z | True} ::RT λ (lq_tmp2 : {lq_tmp2: Z | True}), nilRT)
-             (Z ::UT nilUT)
-             ltac:(mkProjectsArgListTG (({lq_tmp2: Z | True}
-  ::RT λ (lq_tmp2 : {lq_tmp2: Z | True}), nilRT)) ((Z ::UT nilUT)))
-             MaybeInt_u
-             (λ (x_82647028 : ArgList ({lq_tmp2: Z | True} ::RT λ (lq_tmp2 : {lq_tmp2: Z | True}), nilRT))
-                (v_x_82647028 : MaybeInt_u),
-              ltac:(flattenP (λ (lq_tmp2 : {lq_tmp2: Z | True}) (VV : MaybeInt_u),
- MaybeInt_wf VV ∧ True) x_82647028 v_x_82647028))):
-  {VV: _ | bind_rel lq_tmp0 (packProj lq_tmp2) VV}.
-Proof.
-  intros;
-  refine (subsumptionCast
-          _
-          (λ VV, bind_rel lq_tmp0 (packProj lq_tmp2) VV)
-          (bind (exist _ lq_tmp0 lq_tmp0_p) lq_tmp2)
-          _);
-  rewrite <- bind__bind_rel';
-  quicksolve.
-Qed.
-
-#[global] Hint Resolve bind_rel_mk: f_rel_funct_db.
-
-Definition retrn (lq_tmp0 : {lq_tmp0: Z | True}): MaybeInt.
-Proof.
-  destruct lq_tmp0 as [lq_tmp0 lq_tmp0_p]. refine (Just (# lq_tmp0)).
-Defined.
-
-Inductive retrn_rel: Z → MaybeInt_u → Prop :=
-  | retrn_Constr: ∀ lq_tmp0, retrn_rel lq_tmp0 (Just_u lq_tmp0).
-
-#[global] Hint Constructors retrn_rel: core_hint_db.
-
-#[global] Instance retrn_lookup_rel: dictionary rel retrn := { lookup' := retrn_rel }.
-
-#[global] Instance retrn_getF: getFunc retrn_rel := { getF' := retrn }.
-
-Definition retrn_rel_funct [lq_tmp0 : Z]:
-  ∀ (VV VV' : MaybeInt_u), retrn_rel lq_tmp0 VV → (retrn_rel lq_tmp0 VV' → VV = VV').
-Proof.
-  rel_functionhood_body.
-Qed.
-
-#[global] Hint Resolve retrn_rel_funct: f_rel_funct_db.
-
-Theorem retrn_inv_lem lq_tmp0 retrn_inv_lem_res:
-  retrn_rel lq_tmp0 retrn_inv_lem_res ↔ retrn_inv_lem_res == Just_u lq_tmp0.
-Proof.
-  rel_back' _nil.
-Qed.
-
-#[global] Hint Rewrite retrn_inv_lem: f_rel_back.
-
-Theorem retrn_rel_ex (lq_tmp0 : Z) (lq_tmp0_p : True):
-  retrn_rel lq_tmp0 ⌊ retrn (exist _ lq_tmp0 lq_tmp0_p) ⌋.
-Proof.
-  existence_lemma_pre retrn;
-  fix_notations;
-  existence_lemma_quicksolve retrn;
-  f__f_rel_ex_body;
-  f_rel_finish.
-Qed.
-
-#[global] Hint Resolve retrn_rel_ex: rel_ax_db.
-
-Opaque retrn.
-
-Theorem retrn__retrn_rel_rw (lq_tmp0 : Z) (lq_tmp0_p : True) (VV : MaybeInt_u):
-  ⌊ retrn (exist _ lq_tmp0 lq_tmp0_p) ⌋ = VV ↔ retrn_rel lq_tmp0 VV.
-Proof.
-  f__f_rel_rw.
-Qed.
-
-#[global] Hint Rewrite retrn__retrn_rel_rw: f_rel_funct_db.
-
-#[global] Hint Resolve retrn__retrn_rel_rw: rel_ax_db.
-
-#[global] Instance retrn_lookup_rw: dictionary rwLem retrn := { lookup' := retrn__retrn_rel_rw }.
-
-Theorem retrn__retrn_rel (lq_tmp0 : {lq_tmp0: Z | True}) (VV : MaybeInt_u):
-  ⌊ retrn lq_tmp0 ⌋ = VV ↔ retrn_rel ⌊ lq_tmp0 ⌋ VV.
-Proof.
-  f__f_rel.
-Qed.
-
-#[global] Hint Rewrite retrn__retrn_rel: f_rel_funct_db.
-
-Theorem retrn__retrn_rel' (lq_tmp0_u : Z) (lq_tmp0 : {lq_tmp0: Z | True}) (VV : MaybeInt_u):
-  lq_tmp0_u = ⌊ lq_tmp0 ⌋ → ⌊ retrn lq_tmp0 ⌋ = VV ↔ retrn_rel lq_tmp0_u VV.
-Proof.
-  intros ->. refine (retrn__retrn_rel lq_tmp0 VV).
-Qed.
-
-#[global] Hint Resolve retrn__retrn_rel': f_rel_funct_db.
-
-Definition retrn_rel_mk (lq_tmp0 : Z) (lq_tmp0_p : True): {VV: _ | retrn_rel lq_tmp0 VV}.
-Proof.
-  intros;
-  refine (subsumptionCast _ (λ VV, retrn_rel lq_tmp0 VV) (retrn (exist _ lq_tmp0 lq_tmp0_p)) _);
-  rewrite <- retrn__retrn_rel';
-  quicksolve.
-Qed.
-
-#[global] Hint Resolve retrn_rel_mk: f_rel_funct_db.
-
-#[global] Instance retrn_pack:
-  @Pack
-  ({lq_tmp0: Z | True} ::RT λ (lq_tmp0 : {lq_tmp0: Z | True}), nilRT)
-  (Z ::UT nilUT)
-  ltac:(mkProjectsArgListTG (({lq_tmp0: Z | True}
-  ::RT λ (lq_tmp0 : {lq_tmp0: Z | True}), nilRT)) ((Z ::UT nilUT)))
-  MaybeInt_u
-  (λ (x_49697850 : ArgList ({lq_tmp0: Z | True} ::RT λ (lq_tmp0 : {lq_tmp0: Z | True}), nilRT))
-     (v_x_49697850 : MaybeInt_u),
-   ltac:(flattenP (λ (lq_tmp0 : {lq_tmp0: Z | True}) (VV : MaybeInt_u),
- MaybeInt_wf VV ∧ True) x_49697850 v_x_49697850)).
-Proof.
-  buildPackG retrn retrn_rel retrn__retrn_rel retrn_rel_funct.
-Defined.
-
-#[global] Instance retrn_upack: @uPack (Z ::UT nilUT) MaybeInt_u.
-Proof.
-  buildUPackG retrn_rel retrn_rel_funct.
-Defined.
-
-Definition left_identity
-  (x : {x: Z | True})
-  (f : @Pack
-       ({VV: Z | True} ::RT λ (f : {VV: Z | True}), nilRT)
-       (Z ::UT nilUT)
-       ltac:(mkProjectsArgListTG (({VV: Z | True} ::RT λ (f : {VV: Z | True}), nilRT)) ((Z ::UT nilUT)))
-       MaybeInt_u
-       (λ (x_46517173 : ArgList ({VV: Z | True} ::RT λ (f : {VV: Z | True}), nilRT))
-          (v_x_46517173 : MaybeInt_u),
-        ltac:(flattenP (λ (f : {VV: Z | True}) (VV : MaybeInt_u), MaybeInt_wf VV ∧ True) x_46517173 v_x_46517173))):
-  {{∀ retrn_res,
-    retrn_rel ⌊ x ⌋ retrn_res
-    → ∀ bind_res,
-      bind_rel retrn_res ⌊ f ⌋ bind_res → ∀ f_res, getPackRel f ⌊ x ⌋ f_res → bind_res == f_res}}.
-Proof.
-  destruct x as [x x_p].
-  refine (subsumptionCast
-          Unit
-          (λ (VV : Unit),
-           ∀ retrn_res,
-           retrn_rel ⌊ x ⌋ retrn_res
-           → ∀ bind_res,
-             bind_rel retrn_res ⌊ f ⌋ bind_res → ∀ f_res, getPackRel f ⌊ x ⌋ f_res → bind_res == f_res)
-          (# unit)
-          ltac:(solver)).
-Defined.
-
-Definition right_identity (x : MaybeInt):
-  {{∀ bind_res, bind_rel ⌊ x ⌋ retrn_upack bind_res → bind_res == ⌊ x ⌋}}.
-Proof.
-  destruct x as [x x_p].
-  destruct x as [x|].
-  - refine (subsumptionCast
-            Unit
-            (λ (VV : Unit), ∀ bind_res, bind_rel ⌊ x ⌋ retrn_upack bind_res → bind_res == ⌊ x ⌋)
-            (# unit)
-            ltac:(solver)).
-  - refine (subsumptionCast
-            Unit
-            (λ (VV : Unit), ∀ bind_res, bind_rel ⌊ x ⌋ retrn_upack bind_res → bind_res == ⌊ x ⌋)
-            (# unit)
-            ltac:(solver)).
-Defined.
+Definition left_identity_spec (x: {x: Z | True}) (f: (@Pack ({lq_tmp0: Z | True} ::RT (fun (lq_tmp0: {lq_tmp0: Z | True}) => nilRT)) (Z ::UT nilUT) (ltac: (mkProjectsArgListTG ({lq_tmp0: Z | True} ::RT (fun (lq_tmp0: {lq_tmp0: Z | True}) => nilRT)) (Z ::UT nilUT))) MaybeInt_u (fun (x_86410777: (ArgList {lq_tmp0: Z | True} ::RT (fun (lq_tmp0: {lq_tmp0: Z | True}) => nilRT))) => (fun (v_x_86410777: MaybeInt_u) => (ltac: (flattenP (fun (lq_tmp0: {lq_tmp0: Z | True}) => (fun (VV: MaybeInt_u) => ((MaybeInt_wf VV) /\ True))) x_86410777 v_x_86410777)))))): Type := 
+	{{forall (retrnres: MaybeInt_u), (retrn_rel (⌊ x -⌋) retrnres) -> (forall (bindres: MaybeInt_u), (bind_rel retrnres (packProj f) bindres) -> (forall (fres: _), ((getPackRel f) (⌊ x -⌋) fres) -> (bindres == fres)))}}. 
+#[global] Hint Unfold left_identity_spec : lia_unfold.
+Theorem left_identity (x: {x: Z | True}) (f: (@Pack ({lq_tmp0: Z | True} ::RT (fun (lq_tmp0: {lq_tmp0: Z | True}) => nilRT)) (Z ::UT nilUT) (ltac: (mkProjectsArgListTG ({lq_tmp0: Z | True} ::RT (fun (lq_tmp0: {lq_tmp0: Z | True}) => nilRT)) (Z ::UT nilUT))) MaybeInt_u (fun (x_86410777: (ArgList {lq_tmp0: Z | True} ::RT (fun (lq_tmp0: {lq_tmp0: Z | True}) => nilRT))) => (fun (v_x_86410777: MaybeInt_u) => (ltac: (flattenP (fun (lq_tmp0: {lq_tmp0: Z | True}) => (fun (VV: MaybeInt_u) => ((MaybeInt_wf VV) /\ True))) x_86410777 v_x_86410777)))))): left_identity_spec x f. 
+Proof. 
+	destruct x as [x x_p]. 
+	refine (exist _ unit _); 
+	solver. 
+Qed. 
+Definition right_identity_spec (x: MaybeInt): Type := 
+	{{forall (bindres: MaybeInt_u), (bind_rel (⌊ x -⌋) 
+		(ltac: (pose retrn_rel as Rel; 
+	pose retrn_rel_funct as Funct; 
+	buildUPackG Rel Funct)) bindres) -> (bindres = (⌊ x -⌋))}}. 
+#[global] Hint Unfold right_identity_spec : lia_unfold.
+Theorem right_identity (x: MaybeInt): right_identity_spec x. 
+Proof. 
+	destruct x as [x x_p]. 
+	induction x as [(*Just*) x | (*Nothing*) ]. 
+	  - intros . 
+		refine (exist _ unit _); 
+		solver.  
+	  - intros . 
+		refine (exist _ unit _); 
+		solver.  
+Qed. 
