lava/out/Benchmark/PLE/Lambdas.v
@@ -1,29 +1,35 @@
 From coqDeps Require Export LiquidPreludeUtil.
 Open Scope Z_scope.
 Open Scope Int_scope.
-From Coq Require Import Unicode.Utf8.
-Ltac solver := quicksolve.
-
-Definition fvInLambda (x : {x: Z | True}): {VV: Z | True}.
-Proof.
-  destruct x as [x x_p].
-  assert (f_15080524 : ∀ (y : {VV: Z | True}),
-                       {v: Z | ∀ addZ_res, addZ_rel x ⌊ y ⌋ addZ_res → v == addZ_res}).
-  { intros [y y_p];
-    refine (subsumptionCast
-            Z
-            (λ (v : Z), ∀ addZ_res, addZ_rel x ⌊ y ⌋ addZ_res → v == addZ_res)
-            (# x +Z # y)
-            ltac:(solver)). }
-  unshelve refine (let f : ltac:(buildPackG_spec f_15080524) := (ltac:(fun_to_pack f_15080524)) in _).
-  refine (subsumptionCast Z (λ (VV : Z), True) (getPackF f (# x)) ltac:(solver)).
-Defined.
-
-Definition appId (x : {x: Z | True}): {VV: Z | True}.
-Proof.
-  destruct x as [x x_p].
-  assert (f_70768816 : ∀ (y : {VV: Z | True}), {v: Z | v == ⌊ y ⌋}).
-  { intros [y y_p]; refine (subsumptionCast Z (λ (v : Z), v == ⌊ y ⌋) (# y) ltac:(solver)). }
-  unshelve refine (let f : ltac:(buildPackG_spec f_70768816) := (ltac:(fun_to_pack f_70768816)) in _).
-  refine (subsumptionCast Z (λ (VV : Z), True) (getPackF f (# x)) ltac:(solver)).
-Defined.
+Set Universe Polymorphism.
+Definition fvInLambda_spec (x: {x: Z | True}): Type := 
+	{VV: Z | True}. 
+#[global] Hint Unfold fvInLambda_spec : lia_unfold.
+Definition fvInLambda (x: {x: Z | True}): fvInLambda_spec x. 
+Proof. 
+	destruct x as [x x_p]. 
+	assert (f_84163371: (forall (y: {y: Z | True}) , {v: Z | forall (addZres: Z), (addZ_rel x (⌊ y -⌋) addZres) -> (v == addZres)})) by (intros y; 
+	destruct y as [y y_p]; 
+	refine (subsumptionCast _ _ 
+		((exist (fun (x_1: Z) => True) x (ltac: (solver))) +Z (exist (fun (x_2: Z) => True) y (ltac: (solver)))) _); 
+	solver). 
+	unshelve refine (let f : ltac:(buildPackG_spec f_84163371) := (ltac:(fun_to_pack f_84163371)) in _). 
+	refine (subsumptionCast _ _ 
+		((getPackF f) (exist (fun (y: Z) => True) x (ltac: (solver)))) _); 
+	solver. 
+Defined. 
+Definition appId_spec (x: {x: Z | True}): Type := 
+	{VV: Z | True}. 
+#[global] Hint Unfold appId_spec : lia_unfold.
+Definition appId (x: {x: Z | True}): appId_spec x. 
+Proof. 
+	destruct x as [x x_p]. 
+	assert (f_73066757: (forall (y: {y: Z | True}) , {v: Z | v = (⌊ y -⌋)})) by (intros y; 
+	destruct y as [y y_p]; 
+	refine (exist _ y _); 
+	solver). 
+	unshelve refine (let f : ltac:(buildPackG_spec f_73066757) := (ltac:(fun_to_pack f_73066757)) in _). 
+	refine (subsumptionCast _ _ 
+		((getPackF f) (exist (fun (y: Z) => True) x (ltac: (solver)))) _); 
+	solver. 
+Defined. 
